Sketch 'NatRangeIterator' adheres to 'Iterator'
- It turns out we can reduce our 'wf' proposition to a more convenient
  form which directly states facts about the state. We'll do that next
  before continuing.

App/Lib/NatRangeIterator/Spec.v
@@ -1,12 +1,17 @@
+Require Import He4.Language.DynamicBinding.
 Require Import He4.Language.State.
 Require Import He4.Language.StepProp.
+Require Import He4.Language.Term.
 
 Section Specs.
 
 Variable step : step_relation.
 
 Definition wf (st : state) : Prop :=
-  True.
+     called_on_class "NatRangeIterator" st
+  /\ (exists b, multi step (pair (texec "get_at_start") st) (pair (tbool b) st))
+  /\ (exists n, multi step (pair (texec "get_count") st) (pair (tnat n) st))
+  /\ (exists n, multi step (pair (texec "get_first") st) (pair (tnat n) st)).
 
 End Specs.
 
